#+title: do it yourself type theory

* [note]

  - by Roland Backhouse, Paul Chisholm, Erik Saaman and Grant Malcolm, 1988

* 2.2 An Example Derivation

  A type
  ------------------
  { x : A -- x : A }

  { x : A -- f(x) : B }
  ------------------------
  (x) => f(x) : A -> B

  a : A
  f : A -> B
  --------------
  f(x) : B

  a : A
  ----------------
  inl(a) : A + B

  b : B
  ----------------
  inr(b) : A + B

  example proof:

  (f) => f(inr((x) => f(inl(x)))) : ((A + ((A) -> B)) -> B) -> B

  example steps:

  #+begin_src js
  { f : (A + ((A) -> B)) -> B
    ----------
    { x : A
      -----------
      inl(x) : A + ((A) -> B)
      f(inl(x)) : B
    }
    (x) => f(inl(x)) : (A) -> B
    inr((x) => f(inl(x))) : A + ((A) -> B)
    f(inr((x) => f(inl(x)))) : B
  }
  (f) => f(inr((x) => f(inl(x)))) : ((A + ((A) -> B)) -> B) -> B
  #+end_src
